WIP

NuBasicAbstractors.thy
@@ -31,8 +31,8 @@ lemma [simp]: "p \<nuLinkL> Identity \<nuLinkR> x \<longleftrightarrow> p = x" u
 
 subsubsection \<open>Refinement\<close>
 
-definition NuRefine :: " ('a :: lrep, 'b) \<nu> \<Rightarrow> 'b set \<Rightarrow> ('a, 'b) \<nu> " (infixl "\<nuRefine>" 80)
-  where "(N \<nuRefine> T) p x = (x \<in> T \<and>(p \<nuLinkL> N \<nuLinkR> x))"
+definition NuRefine :: " ('a, 'b) \<nu> \<Rightarrow> 'b set \<Rightarrow> ('a, 'b) \<nu> " (infixl "\<nuRefine>" 80)
+  where "(N \<nuRefine> T) x p = (x \<in> T \<and>(p \<nuLinkL> N \<nuLinkR> x))"
 
 notation NuRefine (infixl "<where>" 80)
 
@@ -44,6 +44,9 @@ lemma [\<nu>intro]: "\<^bold>i\<^bold>n\<^bold>t\<^bold>r\<^bold>o \<^bold>c\<^b
 lemma [\<nu>intro]: "\<^bold>d\<^bold>e\<^bold>s\<^bold>t \<^bold>c\<^bold>a\<^bold>s\<^bold>t x \<tycolon> M <where> S \<longmapsto> x \<tycolon> M \<^bold>w\<^bold>i\<^bold>t\<^bold>h x \<in> S"
   unfolding Dest_def Cast_def by auto
 lemma refine_\<nu>cast: "\<^bold>p\<^bold>a\<^bold>r\<^bold>a\<^bold>m P \<Longrightarrow> \<^bold>p\<^bold>r\<^bold>e\<^bold>m\<^bold>i\<^bold>s\<^bold>e x \<in> P \<Longrightarrow> \<^bold>c\<^bold>a\<^bold>s\<^bold>t x \<tycolon> N \<longmapsto> x \<tycolon> (N <where> P)" unfolding Cast_def by auto
+
+lemma [simp,\<nu>auto_expansion]:"\<tort_lbrace>x \<tycolon> Auto NuRefine T P \<tort_rbrace> = \<tort_lbrace> x \<tycolon> Auto NuAddition T (x \<in> P) \<tort_rbrace>"
+  unfolding Auto_def by auto
 
 (* lemma [\<nu>intro]: "(x \<in> P \<Longrightarrow> \<^bold>c\<^bold>a\<^bold>s\<^bold>t x \<tycolon> N \<longmapsto> Y \<^bold>w\<^bold>i\<^bold>t\<^bold>h Q) \<Longrightarrow> \<^bold>c\<^bold>a\<^bold>s\<^bold>t x \<tycolon> N \<nuRefine> P \<longmapsto> Y \<^bold>w\<^bold>i\<^bold>t\<^bold>h Q \<and>x \<in> P" unfolding Cast_def by auto
 lemma [\<nu>intro]: " \<^bold>c\<^bold>a\<^bold>s\<^bold>t x \<tycolon> N \<longmapsto> y \<tycolon> M \<^bold>w\<^bold>i\<^bold>t\<^bold>h Q \<Longrightarrow> \<^bold>p\<^bold>r\<^bold>e\<^bold>m\<^bold>i\<^bold>s\<^bold>e y \<in> P \<Longrightarrow> \<^bold>c\<^bold>a\<^bold>s\<^bold>t x \<tycolon> N \<longmapsto> y \<tycolon> M <where> P \<^bold>w\<^bold>i\<^bold>t\<^bold>h Q" unfolding Cast_def by auto
@@ -64,7 +67,7 @@ lemma refine'_\<nu>cast: "\<^bold>p\<^bold>a\<^bold>r\<^bold>a\<^bold>m P \<Long
 subsubsection \<open>Down Lifting\<close>
 
 definition DownLift :: "('a, 'b) \<nu> \<Rightarrow> ('c \<Rightarrow> 'b) \<Rightarrow> ('a,'c) \<nu>" (infixl "<down-lift>" 80)
-  where "DownLift N g p x = ( p \<nuLinkL> N \<nuLinkR> g x)"
+  where "DownLift N g x p = ( p \<nuLinkL> N \<nuLinkR> g x)"
 
 lemma DownLift_exp[simp]: " p \<nuLinkL> N <down-lift> g \<nuLinkR> x \<longleftrightarrow> p \<nuLinkL> N \<nuLinkR> g x"
   unfolding DownLift_def Refining_ex by simp
@@ -81,6 +84,8 @@ lemma [\<nu>intro]: "\<^bold>d\<^bold>e\<^bold>s\<^bold>t \<^bold>c\<^bold>a\<^b
 lemma [\<nu>intro]: " \<^bold>c\<^bold>a\<^bold>s\<^bold>t x \<tycolon> N \<longmapsto> y1 \<tycolon> M \<^bold>w\<^bold>i\<^bold>t\<^bold>h P \<Longrightarrow> \<^bold>p\<^bold>r\<^bold>e\<^bold>m\<^bold>i\<^bold>s\<^bold>e y1 = g y  \<Longrightarrow> \<^bold>c\<^bold>a\<^bold>s\<^bold>t x \<tycolon> N \<longmapsto> y \<tycolon> M <down-lift> g" unfolding Cast_def by auto
 lemma "\<down>lift_\<nu>cast": "\<^bold>p\<^bold>a\<^bold>r\<^bold>a\<^bold>m g \<Longrightarrow> \<^bold>p\<^bold>r\<^bold>e\<^bold>m\<^bold>i\<^bold>s\<^bold>e g y = x \<Longrightarrow> \<^bold>c\<^bold>a\<^bold>s\<^bold>t x \<tycolon> N \<longmapsto> y \<tycolon> N <down-lift> g" unfolding Cast_def by auto
 
+lemma [simp,\<nu>auto_expansion]:"\<tort_lbrace>x \<tycolon> Auto DownLift T f \<tort_rbrace> = \<tort_lbrace> f x \<tycolon> T \<tort_rbrace>" unfolding Auto_def by auto
+
 (* term image
 lemma "\<nu>Equal (N <down-lift> g) can_eq eq \<longleftrightarrow> \<nu>Equal N (inv_imagep can_eq g) (inv_imagep eq g)"
   unfolding \<nu>Equal_def by auto *)
@@ -94,7 +99,7 @@ lemma [\<nu>intro]: "\<^bold>c\<^bold>a\<^bold>s\<^bold>t x \<tycolon> N \<longm
 subsubsection \<open>Up Lifting\<close>
 
 definition UpLift :: "(('a::lrep), 'c) \<nu> \<Rightarrow> ('c \<Rightarrow> 'b) \<Rightarrow> ('a,'b) \<nu>" (infixl "<up-lift>" 80)
-  where "UpLift N f p x = (\<exists>y. f y = x \<and> ( p \<nuLinkL> N \<nuLinkR> y))"
+  where "UpLift N f x p = (\<exists>y. f y = x \<and> ( p \<nuLinkL> N \<nuLinkR> y))"
 
 lemma [simp]: " p \<nuLinkL> N <up-lift> f \<nuLinkR> x \<longleftrightarrow> (\<exists>y. (f y = x) \<and> (p \<nuLinkL> N \<nuLinkR> y))"
   unfolding UpLift_def Refining_ex by auto
@@ -147,14 +152,14 @@ qed
 subsection \<open>\<nu>-abstraction : DeepModel\<close>
 
 definition DeepModel :: "('a::lrep, 'b) \<nu> \<Rightarrow> (deep_model, 'b) \<nu>"
-  where "DeepModel T p x \<longleftrightarrow> shallowize p \<nuLinkL> T \<nuLinkR> x"
+  where "DeepModel T x p \<longleftrightarrow> shallowize p \<nuLinkL> T \<nuLinkR> x"
 
 lemma [simp]: "deepize p \<nuLinkL> DeepModel T \<nuLinkR> x \<longleftrightarrow> p \<nuLinkL> T \<nuLinkR> x" unfolding DeepModel_def Refining_ex by simp
 
 subsection \<open>\<nu>-abstraction : Ref\<close>
 
 definition Ref  :: "('a::lrep, 'b) \<nu> \<Rightarrow> (heap, nat memaddr \<R_arr_tail> 'b) \<nu>"
-  where "Ref T heap xx \<longleftrightarrow> (case xx of addr \<R_arr_tail> x \<Rightarrow> heap \<^bold>a\<^bold>t addr \<^bold>i\<^bold>s x \<tycolon> T)"
+  where "Ref T xx heap \<longleftrightarrow> (case xx of addr \<R_arr_tail> x \<Rightarrow> heap \<^bold>a\<^bold>t addr \<^bold>i\<^bold>s x \<tycolon> T)"
 
 lemma [simp]: "heap \<nuLinkL> Ref T \<nuLinkR> addr \<R_arr_tail> x \<longleftrightarrow> (heap \<^bold>a\<^bold>t addr \<^bold>i\<^bold>s x \<tycolon> T)"
   by (auto simp add: lrep_exps Ref_def Refining_ex)
@@ -163,7 +168,7 @@ lemma [elim]: " addr \<R_arr_tail> x \<ratio> Ref T \<Longrightarrow> (x \<ratio
 subsection \<open>\<nu>-abstraction : Array'\<close>
 
 definition Array' :: "('a::field, 'b) \<nu> \<Rightarrow> (heap, nat memaddr \<R_arr_tail> 'b option list) \<nu>"
-  where "Array' N heap x' = (case x' of (base |+ ofs) \<R_arr_tail> xs \<Rightarrow>
+  where "Array' N x' heap = (case x' of (base |+ ofs) \<R_arr_tail> xs \<Rightarrow>
     (\<forall>i < length xs. pred_option (\<lambda>x. heap \<^bold>a\<^bold>t base |+ (ofs + i) \<^bold>i\<^bold>s x \<tycolon> N) (xs ! i)) \<and>
     ofs + length xs \<le> segment_len base \<and> segment_llty base = LLTY('a))"
 
@@ -238,7 +243,7 @@ lemma [simp]: "i < length l \<Longrightarrow> the (mapSome l ! i) = l ! i" unfol
 lemma cast_dual_trans: 
   "\<^bold>c\<^bold>a\<^bold>s\<^bold>t A \<longmapsto> B \<^bold>w\<^bold>i\<^bold>t\<^bold>h P1 \<^bold>d\<^bold>u\<^bold>a\<^bold>l B' \<longmapsto> A' \<^bold>w\<^bold>h\<^bold>e\<^bold>n Q1 \<Longrightarrow> \<^bold>c\<^bold>a\<^bold>s\<^bold>t B \<longmapsto> C \<^bold>w\<^bold>i\<^bold>t\<^bold>h P2 \<^bold>d\<^bold>u\<^bold>a\<^bold>l C' \<longmapsto> B' \<^bold>w\<^bold>h\<^bold>e\<^bold>n Q2
     \<Longrightarrow> \<^bold>c\<^bold>a\<^bold>s\<^bold>t A \<longmapsto> C \<^bold>w\<^bold>i\<^bold>t\<^bold>h P1 \<and> P2 \<^bold>d\<^bold>u\<^bold>a\<^bold>l C' \<longmapsto> A' \<^bold>w\<^bold>h\<^bold>e\<^bold>n Q1 \<and> Q2"
-  unfolding Cast_def CastDual_def by auto
+  unfolding Cast_def CastDual_def Intro_def Dest_def by auto
 
 lemma [\<nu>intro]: "\<^bold>i\<^bold>n\<^bold>t\<^bold>r\<^bold>o \<^bold>c\<^bold>a\<^bold>s\<^bold>t  a \<R_arr_tail> xs' \<tycolon> Array' N \<longmapsto> a \<R_arr_tail> xs2 \<tycolon> Array N \<^bold>w\<^bold>h\<^bold>e\<^bold>n xs' = mapSome xs2"
   unfolding Cast_def Intro_def Array_def by (cases a) (auto simp add: pred_option_def Ball_def)
